using abstract component model

working/composition/event_based_refinement/load_balancer/compositional/abstract_composition/ComposedNetwork.t.dfy
@@ -1,32 +1,8 @@
-include "../shared/Types.t.dfy"
-include "ComposedSpec.t.dfy"
-include "../shared/DistributedSystem.t.dfy"
+include "../shared/AbstractNetwork.t.dfy"
+include "ComposedHost.t.dfy"
 
-// analogous to module: AbstractNetwork
-abstract module ComposedNetwork {
-    import opened Types
-    import opened Spec: ComposedSpec
+abstract module ComposedNetwork refines AbstractNetwork {
+    import opened Host: ComposedHost
 
-    datatype ComposedMessage = MessageA(msgA: DSA.Network.Host.Message) | MessageB(msgB: DSB.Network.Host.Message)
-    datatype ComposedMessageOps = MessageOps(recv:Option<ComposedMessage>, send:Option<ComposedMessage>, send_trans:Option<ComposedMessage>)
-
-    ghost predicate TranslateExternalMessages(fromMsg: Option<ComposedMessage>, toMsg: Option<ComposedMessage>) 
-
-    datatype Constants = Constants
-
-    datatype Variables = Variables(sentMsgs:set<ComposedMessage>)
-
-    ghost predicate Init(c: Constants, v: Variables)
-    {
-        && v.sentMsgs == {}
-    }
-
-    ghost predicate Next(c: Constants, v: Variables, v': Variables, msgOps: ComposedMessageOps)
-    {
-        && (msgOps.recv.Some? ==> msgOps.recv.value in v.sentMsgs)
-        && TranslateExternalMessages(msgOps.send, msgOps.send_trans) 
-        && v'.sentMsgs == v.sentMsgs
-            + (if msgOps.send.None? then {} else { msgOps.send.value })
-            + (if msgOps.send_trans.None? then {} else { msgOps.send_trans.value })
-  }
+    // todo -- need to override next!
 }
