working/composition/event_based_refinement/load_balancer/compositional/client_server/ClientServerNetwork.v.dfy
@@ -1,16 +1,6 @@
 include "../abstract_composition/ComposedNetwork.t.dfy"
-include "ClientServerSpec.t.dfy"
+include "ClientServerHost.v.dfy"
 
 module ClientServerNetwork refines ComposedNetwork {
-    import opened Spec = ClientServerSpec
-
-    ghost predicate TranslateExternalMessages(fromMsg: Option<ComposedMessage>, toMsg: Option<ComposedMessage>) 
-    {
-        match fromMsg {
-            case Some(MessageA(ClientRequest(r))) => toMsg == Some(MessageB(Spec.DSB.Network.Host.ServerRequest(r)))
-            case Some(MessageB(ServerResponse(r))) => toMsg == Some(MessageA(Spec.DSA.Network.Host.ClientResponse(r)))
-            case Some(_) => toMsg == None
-            case None => toMsg == None
-        }
-    }
+    import opened Host = ClientServerHost
 }
