working/composition/event_based_refinement/load_balancer/compositional/abstract_composition/ComposedComponent.t.dfy
@@ -1,0 +1,192 @@
+include "../shared/Types.t.dfy"
+include "../shared/AbstractComponent.t.dfy"
+include "ComposedNetwork.t.dfy"
+
+abstract module ComposedComponentDef refines AbstractComponent {
+    import opened Network: ComposedNetwork
+
+    datatype ConstantsImpl = ConstantsImpl(
+        componentA: Host.Spec.ComponentA.Constants,
+        componentB: Host.Spec.ComponentB.Constants) 
+    {
+        ghost predicate WF() 
+        {
+            && componentA.WF()
+            && componentB.WF()
+        }
+    }
+
+    datatype VariablesImpl = VariablesImpl(
+        componentA: Host.Spec.ComponentA.Variables,
+        componentB: Host.Spec.ComponentB.Variables) 
+    {
+        ghost predicate WF(c: ConstantsImpl) {
+            && c.WF()
+            && componentA.WF(c.componentA)
+            && componentB.WF(c.componentB)
+        }
+    }
+
+    ghost predicate Init(c: Constants, v: Variables) {
+        && v.WF(c)
+        && Host.Spec.ComponentA.Init(c.c.componentA, v.v.componentA)
+        && Host.Spec.ComponentB.Init(c.c.componentB, v.v.componentB)
+    }
+
+    ghost predicate IsMessageSetA(msgs: seq<Host.Message>) {
+        || msgs == []
+        || (forall m :: m in msgs ==> m.MessageA?)
+    }
+
+    ghost predicate IsMessageOpsA(msgOps: Host.ComposedMessageOps) 
+    {
+        && IsMessageSetA(msgOps.recv)
+        && IsMessageSetA(msgOps.send)
+    }
+
+    ghost function UnwrapMessageSetA(msgs: seq<Host.Message>) : seq<Host.Spec.ComponentA.Network.Host.Message>
+        requires IsMessageSetA(msgs)
+        ensures |msgs| == |UnwrapMessageSetA(msgs)|
+        ensures forall i :: 0 <= i < |msgs| ==> UnwrapMessageSetA(msgs)[i] == msgs[i].msgA
+    {
+        if msgs == []
+            then []
+            else [msgs[0].msgA] + UnwrapMessageSetA(msgs[1..])
+    }
+
+    ghost function UnwrapMessageOpsA(msgOps: Host.ComposedMessageOps): Host.Spec.ComponentA.Network.Host.MessageOps
+        requires IsMessageOpsA(msgOps)
+    {
+        Host.Spec.ComponentA.Network.Host.MessageOps(
+            UnwrapMessageSetA(msgOps.recv),
+            UnwrapMessageSetA(msgOps.send)
+        )
+    }
+
+    ghost predicate IsTransMessageA(msgOps: Host.ComposedMessageOps) 
+    {
+        IsMessageSetA(msgOps.send_trans)
+    }
+
+    ghost function UnwrapTransMessageOpsA(msgOps: Host.ComposedMessageOps) : Host.Spec.ComponentA.Network.Host.MessageOps
+        requires IsTransMessageA(msgOps)
+    {
+        Host.Spec.ComponentA.Network.Host.MessageOps(
+            [],
+            UnwrapMessageSetA(msgOps.send_trans)
+        )
+    }
+
+    ghost predicate IsMessageSetB(msgs: seq<Host.Message>) {
+        || msgs == []
+        || (forall m :: m in msgs ==> m.MessageB?)
+    }
+
+    ghost predicate IsMessageOpsB(msgOps: Host.ComposedMessageOps) 
+    {
+        && IsMessageSetB(msgOps.recv)
+        && IsMessageSetB(msgOps.send)
+    }
+
+    ghost function UnwrapMessageSetB(msgs: seq<Host.Message>) : seq<Host.Spec.ComponentB.Network.Host.Message>
+        requires IsMessageSetB(msgs)
+        ensures |msgs| == |UnwrapMessageSetB(msgs)|
+        ensures forall i :: 0 <= i < |msgs| ==> UnwrapMessageSetB(msgs)[i] == msgs[i].msgB
+    {
+        if msgs == []
+            then []
+            else [msgs[0].msgB] + UnwrapMessageSetB(msgs[1..])
+    }
+
+    ghost function UnwrapMessageOpsB(msgOps: Host.ComposedMessageOps): Host.Spec.ComponentB.Network.Host.MessageOps
+        requires IsMessageOpsB(msgOps)
+    {
+        Host.Spec.ComponentB.Network.Host.MessageOps(
+            UnwrapMessageSetB(msgOps.recv),
+            UnwrapMessageSetB(msgOps.send)
+        )
+    }
+
+    ghost predicate IsTransMessageB(msgOps: Host.ComposedMessageOps) 
+    {
+        IsMessageSetB(msgOps.send_trans)
+    }
+
+    ghost function UnwrapTransMessageOpsB(msgOps: Host.ComposedMessageOps) : Host.Spec.ComponentB.Network.Host.MessageOps
+        requires IsTransMessageB(msgOps)
+    {
+        Host.Spec.ComponentB.Network.Host.MessageOps(
+            [],
+            UnwrapMessageSetB(msgOps.send_trans)
+        )
+    }
+
+    ghost predicate ComponentAAction(c: Constants, v: Variables, v': Variables, evt: Host.Spec.Event, msgOps: Host.ComposedMessageOps)
+        requires v.WF(c)
+        requires v'.WF(c)
+    {
+        && evt.EventA?
+        && IsMessageOpsA(msgOps)
+        && IsTransMessageB(msgOps)
+        && (exists step :: Host.Spec.ComponentA.Action(c.c.componentA, v.v.componentA, v'.v.componentA, evt.evtA, UnwrapMessageOpsA(msgOps), step))
+        && Host.Spec.ComponentB.ExternalMessageAction(c.c.componentB, v.v.componentB, v'.v.componentB, UnwrapTransMessageOpsB(msgOps))
+    }
+
+    ghost predicate ComponentBAction(c: Constants, v: Variables, v': Variables, evt: Host.Spec.Event, msgOps: Host.ComposedMessageOps)
+        requires v.WF(c)
+        requires v'.WF(c)
+    {
+        && evt.EventB?
+        && IsMessageOpsB(msgOps)
+        && IsTransMessageA(msgOps)
+        && (exists step :: Host.Spec.ComponentB.Action(c.c.componentB, v.v.componentB, v'.v.componentB, evt.evtB, UnwrapMessageOpsB(msgOps), step))
+        && Host.Spec.ComponentA.ExternalMessageAction(c.c.componentA, v.v.componentA, v'.v.componentA, UnwrapTransMessageOpsA(msgOps))
+    }
+
+    ghost predicate ComponentAction(c: Constants, v: Variables, v': Variables, evt: Host.Spec.Event, msgOps: Host.ComposedMessageOps)
+    {
+        && v.WF(c)
+        && v'.WF(c)
+        && (ComponentAAction(c, v, v', evt, msgOps) || ComponentBAction(c, v, v', evt, msgOps))
+        && Host.TranslateExternalMessages(msgOps.send, msgOps.send_trans)
+    }
+
+    datatype ActionStep =
+        | ComponentActionStep(msgOps: Host.ComposedMessageOps)
+    
+    ghost predicate ActionImpl(c: Constants, v: Variables, v': Variables, evt: Host.Spec.Event, msgOps: Host.MessageOps, step: ActionStep)
+    {
+        && ComponentAction(c, v, v', evt, step.msgOps)
+        && msgOps.recv == step.msgOps.recv
+        && msgOps.send == step.msgOps.send + step.msgOps.send_trans
+    }
+}
+
+abstract module ComposedComponent refines ComposedComponentDef {
+
+    ghost function ConstantsAbstraction(c: Constants) : Network.Host.Spec.Constants
+        //requires c.WF()
+    {
+        Host.Spec.Constants(
+            Host.Spec.ComponentA.ConstantsAbstraction(c.c.componentA), 
+            Host.Spec.ComponentB.ConstantsAbstraction(c.c.componentB))
+    }
+
+    ghost function VariablesAbstraction(c: Constants, v: Variables) : Network.Host.Spec.Variables
+        //requires v.WF(c)
+    {
+        Host.Spec.Variables(
+            Host.Spec.ComponentA.VariablesAbstraction(c.c.componentA, v.v.componentA), 
+            Host.Spec.ComponentB.VariablesAbstraction(c.c.componentB, v.v.componentB))
+    }
+
+    ghost predicate InnerInv(c: Constants, v: Variables)
+    {
+        && Host.Spec.ComponentA.Inv(c.c.componentA, v.v.componentA)
+        && Host.Spec.ComponentB.Inv(c.c.componentB, v.v.componentB)
+    }
+
+    lemma InnerInvLemma(c: Constants, v: Variables)
+        requires Inv(c, v)
+        ensures InnerInv(c, v)
+}
