working/composition/event_based_refinement/load_balancer/compositional/abstract_composition/ComposedHost.t.dfy
@@ -1,0 +1,11 @@
+include "../shared/AbstractHost.t.dfy"
+include "ComposedSpec.t.dfy"
+
+abstract module ComposedHost refines AbstractHost {
+    import opened Spec: ComposedSpec
+
+    datatype Message = MessageA(msgA: ComponentA.Network.Host.Message) | MessageB(msgB: ComponentB.Network.Host.Message)
+    datatype ComposedMessageOps = MessageOps(recv: seq<Message>, send: seq<Message>, send_trans: seq<Message>)
+
+    ghost predicate TranslateExternalMessages(fromMsg: seq<Message>, toMsg: seq<Message>) 
+}
