working/composition/event_based_refinement/load_balancer/compositional/client/ClientSpec.t.dfy
@@ -1,4 +1,4 @@
-include "../shared/Spec.t.dfy"
+include "../shared/AbstractSpec.t.dfy"
 
 module ClientSpec refines AbstractSpec {
     datatype Event = SendRequest | ReceiveResponse
