working/composition/event_based_refinement/load_balancer/compositional/client/Network.v.dfy
@@ -1,6 +1,0 @@
-include "ClientHost.v.dfy"
-include "../shared/Network.t.dfy"
-
-module ClientNetwork refines AbstractNetwork {
-    import opened Host = ClientHost
-}
