working/composition/event_based_refinement/load_balancer/compositional/client_server/ClientServerHost.v.dfy
@@ -1,0 +1,17 @@
+include "../abstract_composition/ComposedHost.t.dfy"
+include "ClientServerSpec.t.dfy"
+
+module ClientServerHost refines ComposedHost {
+    import opened Spec = ClientServerSpec
+
+    ghost predicate TranslateExternalMessages(fromMsg: seq<Message>, toMsg: seq<Message>) 
+    {
+        || (fromMsg == [] == toMsg)
+        || (&& |fromMsg| == 1 
+            && match fromMsg[0] {
+                case MessageA(ClientRequest(r)) => toMsg == [MessageB(Spec.ComponentB.Network.Host.ServerRequest(r))]
+                case MessageB(ServerResponse(r)) => toMsg == [MessageA(Spec.ComponentA.Network.Host.ClientResponse(r))]
+                case _ => toMsg == []
+        })
+    }
+}
