working/composition/event_based_refinement/load_balancer/compositional/client_server/ClientServerRefinementProof.v.dfy
@@ -7,20 +7,20 @@ module ClientServerRefinementProof refines ClientServerDistributedSystem {
         requires v.WF(c)
     {
         forall msg :: 
-            && msg in v.network.sentMsgs 
-            && msg.MessageB?
-            && msg.msgB.ServerRequest? ==> 
-            MessageA(Spec.DSA.Network.Host.ClientRequest(msg.msgB.request)) in v.network.sentMsgs
+            && msg in v.dsB.network.sentMsgs 
+            && msg.ServerRequest? ==> 
+            && Spec.DSA.Network.Host.ClientRequest(msg.request) in v.dsA.network.sentMsgs
+            && Network.TranslateExternalMessages(Some(MessageA(Spec.DSA.Network.Host.ClientRequest(msg.request))), Some(MessageB(msg)))
     }
 
     ghost predicate Inv_ServerResponseClientResponse(c: Constants, v: Variables) 
         requires v.WF(c)
     {
         forall msg :: 
-            && msg in v.network.sentMsgs 
-            && msg.MessageA?
-            && msg.msgA.ClientResponse? ==> 
-            MessageB(Spec.DSB.Network.Host.ServerResponse(msg.msgA.response)) in v.network.sentMsgs
+            && msg in v.dsA.network.sentMsgs 
+            && msg.ClientResponse? ==> 
+            && Spec.DSB.Network.Host.ServerResponse(msg.response) in v.dsB.network.sentMsgs
+            && Network.TranslateExternalMessages(Some(MessageB(Spec.DSB.Network.Host.ServerResponse(msg.response))), Some(MessageA(msg)))
     }
 
     ghost predicate LiftedInv(c: Constants, v: Variables)
@@ -34,19 +34,26 @@ module ClientServerRefinementProof refines ClientServerDistributedSystem {
         // requires LiftedInv(c, v)
         // ensures Inv(c, v)
     {}
+
+    lemma InvInductiveBase(c: Constants, v: Variables)
+        // requires Init(c, v)
+        // ensures LiftedInv(c, v)
+    {}
+
+    lemma InvInductiveNext(c: Constants, v: Variables, v': Variables, evt: Option<Spec.Event>)
+        // requires Next(c, v, v', evt)
+        // requires LiftedInv(c, v)
+        // ensures LiftedInv(c, v')
+    {}
     
     lemma RefinementInit(c: Constants, v: Variables)
-//        requires DistributedSystem.Init(c, v)
-//        ensures LiftedInv(c, v)
+//        requires Init(c, v)
 //        ensures Spec.Init(ConstantsAbstraction(c), VariablesAbstraction(c, v))
-    {
-    }
+    {}
 
     lemma RefinementNext(c: Constants, v: Variables, v': Variables, evt: Option<Spec.Event>)
-//        requires DistributedSystem.Next(c, v, v', evt)
+//        requires Next(c, v, v', evt)
 //        requires LiftedInv(c, v)
-//        ensures LiftedInv(c, v') 
 //        ensures Spec.Next(ConstantsAbstraction(c), VariablesAbstraction(c, v), VariablesAbstraction(c, v'), evt) || (VariablesAbstraction(c, v) == VariablesAbstraction(c, v') && evt == NoOp)
-    {
-    }
+    {}
 }
