working/composition/event_based_refinement/load_balancer/compositional/client_server/ClientServerSpec.t.dfy
@@ -3,6 +3,6 @@ include "../client/RefinementProof.v.dfy"
 include "../server/RefinementProof.v.dfy"
 
 module ClientServerSpec refines ComposedSpec {
-    import DSA = ClientRefinementProof
-    import DSB = ServerRefinementProof
+    import ComponentA = ClientComponent
+    import ComponentB = ServerComponent
 }
