working/composition/event_based_refinement/load_balancer/compositional/server/ServerComponent.v.dfy
@@ -1,8 +1,12 @@
-include "../shared/DistributedSystem.t.dfy"
-include "../shared/RefinementObligation.t.dfy"
-include "Network.v.dfy"
+include "../shared/AbstractSingleComponent.t.dfy"
+include "../shared/AbstractNetwork.t.dfy"
+include "ServerHost.v.dfy"
 
-module ServerDistributedSystem refines RefinementTheorem {
+module ServerNetwork refines AbstractNetwork {
+    import opened Host = ServerHost
+}
+
+module ServerComponentDef refines AbstractSingleComponent {
     import opened Network = ServerNetwork
 
     ghost predicate ValidNext(c: Constants, v: Variables, v': Variables)
@@ -12,7 +16,7 @@ module ServerDistributedSystem refines RefinementTheorem {
 
     ghost predicate NetworkStep(c: Constants, v: Variables, v': Variables, evt: Option<Host.Spec.Event>)
     {
-        exists step: Step :: step.NetworkActionStep? && NetworkAction(c, v, v', evt, step.msgOps)
+        exists step: Step :: step.ExternalMessageActionStep? && ExternalMessageAction(c, v, v', step.msgOps)
     }
 
     ghost predicate ExistsRequestMessage(c: Constants, prefix: seq<Variables>, i: nat)
@@ -24,10 +28,8 @@ module ServerDistributedSystem refines RefinementTheorem {
     ghost predicate RequestMessage(c: Constants, prefix: seq<Variables>, i: nat, msgOps: Host.MessageOps)
         requires |prefix| > i + 1
     {
-        && NetworkAction(c, prefix[i], prefix[i+1], None, msgOps) 
-        && msgOps.send.Some?
-        && msgOps.send.value.ServerRequest?
-        && msgOps.send.value.request.seqNo == 0
+        && ExternalMessageAction(c, prefix[i], prefix[i+1], msgOps) 
+        && exists m :: msgOps.send == [m] && m.ServerRequest? && m.request.seqNo == 0
     }
 
     ghost predicate NonTriviality_PrefixSpec(c: Constants, prefix: seq<Variables>)
@@ -46,16 +48,16 @@ module ServerDistributedSystem refines RefinementTheorem {
         && behavior[0..|prefix|] == prefix
         && (forall i:nat | 0 <= i < |behavior|-1 :: ValidNext(c, behavior[i], behavior[i+1]))
         && behavior[|behavior|-1].WF(c) 
-        && |behavior[|behavior|-1].hosts[0].requests| == |behavior[|behavior|-1].hosts[0].responses| == 1
+        && |behavior[|behavior|-1].v.hosts[0].requests| == |behavior[|behavior|-1].v.hosts[0].responses| == 1
     }
 
     lemma NoOpsPreserveState(c: Constants, start: nat, behavior: seq<Variables>)
         requires forall i:nat | start <= i < |behavior| - 1 :: NetworkStep(c, behavior[i], behavior[i+1], None)
         requires |behavior| - start >= 2
         decreases |behavior| - start
-        ensures forall i, j: nat | start <= i < j < |behavior| - 1 :: behavior[i].hosts ==  behavior[j].hosts
+        ensures forall i, j: nat | start <= i < j < |behavior| - 1 :: behavior[i].v.hosts ==  behavior[j].v.hosts
     {
-        assert behavior[start].hosts == behavior[start+1].hosts;
+        assert behavior[start].v.hosts == behavior[start+1].v.hosts;
         if (|behavior| - start > 2)
         {
             NoOpsPreserveState(c, start + 1, behavior);
@@ -68,7 +70,7 @@ module ServerDistributedSystem refines RefinementTheorem {
         ensures forall i:nat | 0 <= i < |behavior| - 1 :: ValidNext(c, behavior[i], behavior[i+1])
     {
         assert NetworkStep(c, behavior[0], behavior[1], None);
-        var step: Step :| step.NetworkActionStep? && NetworkAction(c, behavior[0], behavior[1], None, step.msgOps);
+        var step: Step :| step.ExternalMessageActionStep? && ExternalMessageAction(c, behavior[0], behavior[1], step.msgOps);
         assert NextStep(c, behavior[0], behavior[1], None, step);
         if (|behavior| > 2) {
             NetworkStepsAreValidSteps(c, behavior[1..]);
@@ -85,23 +87,24 @@ module ServerDistributedSystem refines RefinementTheorem {
         assert (forall i:nat | 0 <= i < |behavior| - 1 :: ValidNext(c, behavior[i], behavior[i+1]));
 
         var msgOps :| RequestMessage(c, prefix, |prefix| - 2, msgOps);
-        var recv := msgOps.send.value;
-        var sum := recv.request.val.0 + recv.request.val.1;
-        var resp := ServiceResponse(recv.request.seqNo, sum);
-        var sent := Host.ServerResponse(resp);
-        msgOps := Host.MessageOps(Some(recv), Some(sent));
+        var m :| msgOps.send == [m] && m.ServerRequest? && m.request.seqNo == 0;
+        var recv := msgOps.send;
+        var sum := m.request.val.0 + m.request.val.1;
+        var resp := ServiceResponse(m.request.seqNo, sum);
+        var sent := [ Host.ServerResponse(resp) ];
+        msgOps := Host.MessageOps(recv, sent);
         behavior := behavior + [Variables.Variables(
-            [
-                Host.Variables([recv.request], [resp])
-            ],
-            Network.Variables(prefix[|prefix|-1].network.sentMsgs + {sent})
+            VariablesImpl([
+                Host.Variables([m.request], [resp])
+            ]),
+            Network.Variables(prefix[|prefix|-1].network.sentMsgs + sent)
         )];
         var i := |behavior| - 2;
         NoOpsPreserveState(c, 0, prefix);
-        assert |prefix[i].hosts[0].requests| == |prefix[i].hosts[0].responses| == 0;
+        assert |prefix[i].v.hosts[0].requests| == |prefix[i].v.hosts[0].responses| == 0;
         assert prefix[i] == behavior[i];
-        assert Host.Compute(c.hosts[0], behavior[i].hosts[0], behavior[i+1].hosts[0], Some(Host.Spec.Compute), msgOps);
-        assert NextStep(c, behavior[i], behavior[i+1], Some(Host.Spec.Compute), HostActionStep(0, msgOps));
+        assert Host.Compute(c.c.hosts[0], behavior[i].v.hosts[0], behavior[i+1].v.hosts[0], Host.Spec.Compute, msgOps);
+        assert NextStep(c, behavior[i], behavior[i+1], Some(Host.Spec.Compute), ActionStep(HostActionStep(0), msgOps));
         assert Next(c, behavior[i], behavior[i+1], Some(Host.Spec.Compute));
     }
 }
