working/composition/event_based_refinement/load_balancer/compositional/shared/AbstractComponent.t.dfy
@@ -1,0 +1,101 @@
+include "Types.t.dfy"
+include "AbstractNetwork.t.dfy"
+
+abstract module AbstractComponentDef {
+    import opened Types
+    import opened Network : AbstractNetwork
+
+    type ConstantsImpl
+    {
+        ghost predicate WF() 
+    }
+
+    datatype Constants = Constants(c: ConstantsImpl, network: Network.Constants)
+    {
+        ghost predicate WF()
+        {
+            c.WF()
+        }
+    }
+
+    type VariablesImpl
+    {
+        ghost predicate WF(c: ConstantsImpl)
+    }
+
+    datatype Variables = Variables(v: VariablesImpl, network: Network.Variables)
+    {
+        ghost predicate WF(c: Constants)
+        {
+            v.WF(c.c)
+        }
+    }
+
+    ghost predicate Init(c: Constants, v: Variables)
+
+    type ActionStep(!new)
+
+    datatype Step = 
+        | ExternalMessageActionStep(msgOps: Host.MessageOps)
+        | ActionStep(actionStep: ActionStep, msgOps: Host.MessageOps)
+
+    ghost predicate ActionImpl(c: Constants, v: Variables, v': Variables, evt: Host.Spec.Event, msgOps: Host.MessageOps, step: ActionStep)
+
+    ghost predicate Action(c: Constants, v: Variables, v': Variables, evt: Host.Spec.Event, msgOps: Host.MessageOps, step: ActionStep)
+    {
+        && v.WF(c)
+        && v'.WF(c)
+        && Network.Next(c.network, v.network, v'.network, msgOps)
+        && ActionImpl(c, v, v', evt, msgOps, step)
+    }
+
+    ghost predicate ExternalMessageAction(c: Constants, v: Variables, v': Variables, msgOps: Host.MessageOps)
+    {
+        && v.WF(c)
+        && v'.WF(c)
+        && (msgOps.send == [] || Host.ExternalMessageSend(msgOps.send))
+        && v.v == v'.v
+        && Network.Next(c.network, v.network, v'.network, msgOps)
+    }
+
+    ghost predicate NextStep(c: Constants, v: Variables, v': Variables, evt: Option<Host.Spec.Event>, step: Step)
+    {
+        || (evt.None? && step.ExternalMessageActionStep? && ExternalMessageAction(c, v, v', step.msgOps))
+        || (evt.Some? && step.ActionStep? && Action(c, v, v', evt.value, step.msgOps, step.actionStep))
+    }
+
+    ghost predicate Next(c: Constants, v: Variables, v': Variables, evt: Option<Host.Spec.Event>)
+    {
+        exists step :: NextStep(c, v, v', evt, step)
+    }
+}
+
+abstract module AbstractComponent refines AbstractComponentDef {
+    ghost function ConstantsAbstraction(c: Constants) : Network.Host.Spec.Constants
+        requires c.WF()
+
+    ghost function VariablesAbstraction(c: Constants, v: Variables) : Network.Host.Spec.Variables
+        requires v.WF(c)
+
+    ghost predicate Inv(c: Constants, v: Variables)
+
+    lemma InvInductiveBase(c: Constants, v: Variables)
+        requires Init(c, v)
+        ensures Inv(c, v)
+
+    lemma InvInductiveNext(c: Constants, v: Variables, v': Variables, evt: Option<Network.Host.Spec.Event>)
+        requires Next(c, v, v', evt)
+        requires Inv(c, v)
+        ensures Inv(c, v')
+
+    lemma RefinementInit(c: Constants, v: Variables)
+        requires Init(c, v)
+        requires c.WF() && v.WF(c)
+        ensures Network.Host.Spec.Init(ConstantsAbstraction(c), VariablesAbstraction(c, v))
+    
+    lemma RefinementNext(c: Constants, v: Variables, v': Variables, evt: Option<Network.Host.Spec.Event>)
+        requires Next(c, v, v', evt)
+        requires Inv(c, v)
+        requires c.WF() && v.WF(c) && v'.WF(c)
+        ensures (evt.Some? && Network.Host.Spec.Next(ConstantsAbstraction(c), VariablesAbstraction(c, v), VariablesAbstraction(c, v'), evt.value)) || (evt.None? && VariablesAbstraction(c, v) == VariablesAbstraction(c, v'))
+}
