working/composition/event_based_refinement/load_balancer/compositional/shared/AbstractSingleComponent.t.dfy
@@ -1,0 +1,46 @@
+include "Types.t.dfy"
+include "AbstractNetwork.t.dfy"
+include "AbstractComponent.t.dfy"
+
+abstract module AbstractSingleComponent refines AbstractComponent {
+    datatype ConstantsImpl = ConstantsImpl(hosts: seq<Host.Constants>) 
+    {
+        ghost predicate WF() 
+        {
+            Host.GroupWFConstants(hosts)
+        }
+    }
+
+    datatype VariablesImpl = VariablesImpl(hosts: seq<Host.Variables>) 
+    {
+        ghost predicate WF(c: ConstantsImpl) {
+            && c.WF()
+            && |c.hosts| == |hosts|
+            && Host.GroupWFVariables(c.hosts, hosts)
+        }
+    }
+
+    ghost predicate Init(c: Constants, v: Variables) {
+        && v.WF(c)
+        && (forall i :: 0 <= i < |c.c.hosts| ==> Host.Init(c.c.hosts[i], v.v.hosts[i]))
+        && Network.Init(c.network, v.network)
+    }
+
+    datatype ActionStep =
+        | HostActionStep(hostId: nat)
+
+    ghost predicate HostAction(c: Constants, v: Variables, v': Variables, evt: Host.Spec.Event, hostId: nat, msgOps: Host.MessageOps)
+    {
+        && v.WF(c)
+        && v'.WF(c)
+        && 0 <= hostId < |v.v.hosts|
+        && Host.Next(c.c.hosts[hostId], v.v.hosts[hostId], v'.v.hosts[hostId], evt, msgOps)
+        && (forall i :: 0 <= i < |v.v.hosts| && i != hostId ==> v.v.hosts[i] == v'.v.hosts[i])
+        && Network.Next(c.network, v.network, v'.network, msgOps)
+    }
+
+    ghost predicate ActionImpl(c: Constants, v: Variables, v': Variables, evt: Host.Spec.Event, msgOps: Host.MessageOps, step: ActionStep)
+    {
+        && HostAction(c, v, v', evt, step.hostId, msgOps)
+    }
+}
